lib/expr: Initial implementation of a reifying compiler for expressions

src/Rupicola/Lib/Compiler.v
@@ -3,7 +3,7 @@ Require Import Rupicola.Lib.Notations.
 Require Export Rupicola.Lib.Gensym.
 Require Import Rupicola.Lib.Tactics.
 
-Section with_parameters.
+Section CompilerBasics.
   Context {semantics : Semantics.parameters}
           {semantics_ok : Semantics.parameters_ok _}.
 
@@ -535,6 +535,391 @@ Section with_parameters.
     all: destruct_one_match; try congruence; [ ]; intros.
     all: eapply compile_seq; eauto.
   Qed.
+End CompilerBasics.
+
+Ltac map_to_list' m :=
+  let rec loop m acc :=
+      match m with
+      | map.put ?m ?k ?v =>
+        loop m uconstr:((k, v) :: acc)
+      | map.empty =>
+        (* Reverse for compatibility with map.of_list *)
+        uconstr:(List.rev_acc acc [])
+      end in
+  loop m uconstr:([]).
+
+Ltac map_to_list m :=
+  let l := map_to_list' m in
+  let l := (eval cbv [List.rev_acc List.app] in l) in
+  l.
+
+Ltac _change x y :=
+  change x with y.
+  (* let Heq := constr:(eq_refl x: x = y) in *)
+  (* replace x with y by (vm_cast_no_check Heq). *)
+
+Tactic Notation "_change_hook" open_constr(x) open_constr(y) :=
+  (_change x y).
+
+Module ExprReflection.
+  Section with_parameters.
+    Context {semantics : Semantics.parameters}
+            {semantics_ok : Semantics.parameters_ok _}.
+
+    Section Core.
+      Class expr_reifier T :=
+        { er_T2w: T -> word;
+          er_default: T;
+          er_op: Type;
+          er_opfun: er_op -> T -> T -> T;
+          er_opname: er_op -> bopname.bopname;
+          er_opfun_morphism: forall op (x y: T),
+              er_T2w ((er_opfun op) x y) =
+              Semantics.interp_binop (er_opname op) (er_T2w x) (er_T2w y) }.
+
+      Context {T} {er: expr_reifier T}.
+
+      Inductive AST :=
+      | ELit (z: Z) (t: T) (ok: option (word.of_Z z = er_T2w t))
+      | EVar (nm: string)
+      | EOp (op: er_op) (l r: AST).
+
+      Context (locals: Semantics.locals)
+              (concrete_locals: map.rep (map := SortedListString.map T)).
+
+      Fixpoint interp ast :=
+        match ast with
+        | ELit z t _ => t
+        | EVar nm => match map.get concrete_locals nm with
+                    | Some v => v
+                    | None => er_default
+                    end
+        | EOp op l r => (er_opfun op) (interp l) (interp r)
+        end.
+
+      Fixpoint compile ast :=
+        match ast with
+        | ELit z t _ => expr.literal z
+        | EVar nm => expr.var nm
+        | EOp op l r => expr.op (er_opname op) (compile l) (compile r)
+        end.
+
+      Definition is_some {A} (o: option A) :=
+        if o then true else false.
+
+      Fixpoint witness ast :=
+        match ast with
+        | ELit _ _ (Some _) => True
+        | ELit z t None => word.of_Z z = er_T2w t
+        | EVar nm => map.get concrete_locals nm <> None
+        | EOp op l r => witness r /\ witness l
+        end.
+
+      Fixpoint witnessb ast acc :=
+        match ast with          (* FIXME use naive word representation for equality checks *)
+        | ELit _ _ (Some _) => acc
+        | ELit z t None => (word.eqb (word.of_Z z) (er_T2w t) && acc)
+        | EVar nm => is_some (map.get concrete_locals nm) && acc
+        | EOp op l r => witnessb r (witnessb l acc)
+        end%bool.
+
+      Lemma witnessb_decreasing ast :
+        witnessb ast false = false.
+      Proof.
+        induction ast; cbn; intros; rewrite ?Bool.andb_false_r.
+        - destruct ok; eauto.
+        - reflexivity.
+        - congruence.
+      Qed.
+
+      Lemma witnessb_sound ast :
+        witnessb ast true = true ->
+        witness ast.
+      Proof.
+        induction ast; cbn; intros H; rewrite ?Bool.andb_true_r in H.
+        - destruct ok; eauto using word.eqb_true.
+        - destruct lookup; cbn in *; congruence.
+        - destruct (witnessb ast1 true); [ solve [eauto] | ].
+          rewrite witnessb_decreasing in H; discriminate.
+      Qed.
+
+      Lemma interp_sound' ast:
+        forall (P: word -> Prop) mem,
+          witness ast ->
+          P (er_T2w (interp ast)) ->
+          map.mapped_compat er_T2w concrete_locals locals ->
+          WeakestPrecondition.expr mem locals (compile ast) P.
+      Proof.
+        induction ast; cbn -[map.get]; intros P mem Hw HP Heq.
+        - destruct ok; red; unfold dlet; congruence.
+        - specialize (Heq nm); destruct map.get.
+          + red; eauto.
+          + exfalso; apply Hw; reflexivity.
+        - apply IHast1; intuition.
+          apply IHast2; intuition.
+          rewrite <- er_opfun_morphism.
+          congruence.
+      Qed.
+
+      Lemma interp_sound ast mem:
+        witnessb ast true = true ->
+        map.mapped_compat er_T2w concrete_locals locals ->
+        WeakestPrecondition.dexpr mem locals (compile ast) (er_T2w (interp ast)).
+      Proof.
+        intros; apply interp_sound'; eauto using witnessb_sound.
+      Qed.
+
+      Lemma interp_complete ast:
+        forall (P: word -> Prop) mem,
+          witness ast ->
+          map.mapped_compat er_T2w concrete_locals locals ->
+          WeakestPrecondition.expr mem locals (compile ast) P ->
+          P (er_T2w (interp ast)).
+      Proof.
+        induction ast; cbn -[map.get]; intros P mem H Heq HP; red in HP.
+        - destruct ok; unfold dlet in HP; congruence.
+        - destruct HP as (x & Heq' & HP).
+          destruct map.get eqn:?.
+          + erewrite Heq in Heq' by eassumption.
+            inversion Heq'; subst; eassumption.
+          + exfalso. eapply H; reflexivity.
+        - destruct H.
+          rewrite er_opfun_morphism.
+          eapply IHast2; intuition.
+          eapply IHast1; intuition.
+          eassumption.
+      Qed.
+    End Core.
+
+    Instance expr_word_reifier : expr_reifier word :=
+      {| er_T2w w := w;
+         er_default := word.of_Z 0;
+         er_op := bopname.bopname;
+         er_opname op := op;
+         er_opfun op :=
+           match op with
+           | bopname.add => word.add
+           | bopname.sub => word.sub
+           | bopname.mul => word.mul
+           | bopname.mulhuu => word.mulhuu
+           | bopname.divu => word.divu
+           | bopname.remu => word.modu
+           | bopname.and => word.and
+           | bopname.or => word.or
+           | bopname.xor => word.xor
+           | bopname.sru => word.sru
+           | bopname.slu => word.slu
+           | bopname.srs => word.srs
+           | bopname.lts => fun x y => b2w (word.lts x y)
+           | bopname.ltu => fun x y => b2w (word.ltu x y)
+           | bopname.eq => fun x y => b2w (word.eqb x y)
+           end;
+         er_opfun_morphism :=
+           ltac:(destruct op; intros; cbn;
+                repeat match goal with
+                       | [  |- context[if ?x then _ else _] ] => destruct x
+                       | _ => reflexivity
+                       end) |}.
+
+    Inductive ReifiedZOpp := RZ_add | RZ_sub | RZ_mul | RZ_land | RZ_lor | RZ_lxor.
+
+    Instance expr_Z_reifier : expr_reifier Z :=
+      {| er_T2w z := word.of_Z z;
+         er_default := 0%Z;
+         er_op := ReifiedZOpp;
+         er_opname zop :=
+           match zop with
+           | RZ_add => bopname.add
+           | RZ_sub => bopname.sub
+           | RZ_mul => bopname.mul
+           | RZ_land => bopname.and
+           | RZ_lor => bopname.or
+           | RZ_lxor => bopname.xor
+           end;
+         er_opfun zop :=
+           match zop with
+           | RZ_add => Z.add
+           | RZ_sub => Z.sub
+           | RZ_mul => Z.mul
+           | RZ_land => Z.land
+           | RZ_lor => Z.lor
+           | RZ_lxor => Z.lxor
+           end;
+         er_opfun_morphism :=
+           ltac:(destruct op; intros; cbn;
+                eauto using word.morph_and, word.morph_or, word.morph_xor,
+                word.ring_morph_add, word.ring_morph_mul, word.ring_morph_sub;
+                reflexivity) |}.
+
+    Lemma compile_expr_w {tr mem locals functions} (v: word) (e: expr) :
+      let v := v in
+      forall {P} {pred: P v -> predicate}
+        {k: nlet_eq_k P v} {k_impl}
+        var,
+        WeakestPrecondition.dexpr mem locals e v ->
+        (let v := v in
+         <{ Trace := tr;
+            Memory := mem;
+            Locals := map.put locals var v;
+            Functions := functions }>
+         k_impl
+         <{ pred (k v eq_refl) }>) ->
+        <{ Trace := tr;
+           Memory := mem;
+           Locals := locals;
+           Functions := functions }>
+        cmd.seq (cmd.set var e) k_impl
+        <{ pred (nlet_eq [var] v k) }>.
+    Proof. repeat straightline; eauto. Qed.
+
+    Lemma compile_expr_Z {tr mem locals functions} (z: Z) (e: expr) :
+      let v := z in
+      forall {P} {pred: P v -> predicate}
+        {k: nlet_eq_k P v} {k_impl}
+        var,
+        WeakestPrecondition.dexpr mem locals e (word.of_Z v) ->
+        (let v := v in
+         <{ Trace := tr;
+            Memory := mem;
+            Locals := map.put locals var (word.of_Z v);
+            Functions := functions }>
+         k_impl
+         <{ pred (k v eq_refl) }>) ->
+        <{ Trace := tr;
+           Memory := mem;
+           Locals := locals;
+           Functions := functions }>
+        cmd.seq (cmd.set var e) k_impl
+        <{ pred (nlet_eq [var] v k) }>.
+    Proof. repeat straightline; eauto. Qed.
+  End with_parameters.
+
+  Ltac find_key_by_value bs v0 :=
+    match bs with
+    | [] => constr:(@None string)
+    | (?k, ?v) :: ?bs =>
+      match v with
+      | v0 => constr:(Some k)
+      | _ => find_key_by_value bs v0
+      end
+    end.
+
+  Ltac expr_reify_word bindings w :=
+    let expr_reify_op nm l r :=
+        let l := expr_reify_word bindings l in
+        let r := expr_reify_word bindings r in
+        constr:(EOp (er := expr_word_reifier) nm l r) in
+    lazymatch w with
+    | word.add ?l ?r    => expr_reify_op bopname.add l r
+    | word.sub ?l ?r    => expr_reify_op bopname.sub l r
+    | word.mul ?l ?r    => expr_reify_op bopname.mul l r
+    | word.mulhuu ?l ?r => expr_reify_op bopname.mulhuu l r
+    | word.divu ?l ?r   => expr_reify_op bopname.divu l r
+    | word.modu ?l ?r   => expr_reify_op bopname.remu l r
+    | word.and ?l ?r    => expr_reify_op bopname.and l r
+    | word.or ?l ?r     => expr_reify_op bopname.or l r
+    | word.xor ?l ?r    => expr_reify_op bopname.xor l r
+    | word.sru ?l ?r    => expr_reify_op bopname.sru l r
+    | word.slu ?l ?r    => expr_reify_op bopname.slu l r
+    | word.srs ?l ?r    => expr_reify_op bopname.srs l r
+    | word.lts ?l ?r    => expr_reify_op bopname.lts l r
+    | word.ltu ?l ?r    => expr_reify_op bopname.ltu l r
+    | word.eqb ?l ?r    => expr_reify_op bopname.eq l r
+    | _ =>
+      lazymatch find_key_by_value bindings w with
+      | Some ?k => constr:(EVar (er := expr_word_reifier) k)
+      | None =>
+        lazymatch w with
+        | word.of_Z ?z => constr:(ELit (er := expr_word_reifier) z (word.of_Z z) (Some eq_refl))
+        | _ => constr:(ELit (er := expr_word_reifier) (word.unsigned w) w None)
+        end
+      end
+    end.
+
+  Ltac expr_reify_Z bindings z :=
+    let expr_reify_op nm l r :=
+        let l := expr_reify_Z bindings l in
+        let r := expr_reify_Z bindings r in
+        constr:(EOp (er := expr_Z_reifier) nm l r) in
+    lazymatch z with
+    | Z.add ?l ?r  => expr_reify_op RZ_add l r
+    | Z.sub ?l ?r  => expr_reify_op RZ_sub l r
+    | Z.mul ?l ?r  => expr_reify_op RZ_mul l r
+    | Z.land ?l ?r => expr_reify_op RZ_land l r
+    | Z.lor ?l ?r  => expr_reify_op RZ_lor l r
+    | Z.lxor ?l ?r => expr_reify_op RZ_lxor l r
+    | _ =>
+      lazymatch find_key_by_value bindings z with
+      | Some ?k => constr:(EVar (er := expr_Z_reifier) k)
+      | None => constr:(ELit (er := expr_Z_reifier) z z (Some eq_refl))
+      end
+    end.
+
+  Ltac compile_reified_expr_w locals w :=
+    let bindings := map_to_list locals in
+    let reified := expr_reify_word bindings w in
+    simple apply compile_expr_w with (e := compile reified);
+    [ change locals with (map.of_list bindings);
+      _change_hook w (er_T2w (expr_reifier := expr_word_reifier)
+                             (interp (map.of_list (map := SortedListString.map _) bindings) reified))
+    | ].
+
+  Ltac zify_bindings bs :=
+    match bs with
+    | [] => constr:(@List.nil (string * Z))
+    | (?k, ?w) :: ?tl =>
+      let z := match w with
+              | @word.of_Z _ _ ?z => constr:(z)
+              | _                 => constr:(word.unsigned w)
+              end in
+      let tl := zify_bindings tl in
+      constr:((k, z) :: tl)
+    end.
+
+  Ltac compile_reified_expr_Z locals z :=
+    let bindings := map_to_list locals in
+    let z_bindings := zify_bindings bindings in
+    let z_bindings := type_term z_bindings in
+    let reified := ExprReflection.expr_reify_Z z_bindings z in
+    simple apply compile_expr_Z with (e := ExprReflection.compile reified);
+    [ change locals with (map.of_list bindings);
+      _change_hook (word.of_Z z)
+                   (ExprReflection.er_T2w
+                      (expr_reifier := expr_Z_reifier)
+                      (ExprReflection.interp (er := expr_Z_reifier)
+                                             (map.of_list (map := SortedListString.map _) z_bindings)
+                                             reified))
+    | ].
+
+  Ltac compile_prove_expr_reification_premise :=
+    eapply interp_sound;
+    [ reflexivity |
+      apply map.mapped_compat_of_list;
+      lazymatch goal with
+      | |- context[expr_Z_reifier] => (* LATER Use reification to speed up this rewrite *)
+        cbv [List.map fst snd er_T2w expr_Z_reifier]; rewrite ?word.of_Z_unsigned
+      | _ => idtac
+      end; reflexivity
+      | .. ].
+
+  Ltac compile_apply_expr_reification_lemma :=
+    lazymatch goal with
+    | [ |- WeakestPrecondition.cmd _ _ _ _ ?locals (_ (nlet_eq _ ?v _)) ] =>
+      lazymatch type of v with
+      | word.rep => compile_reified_expr_w locals v
+      | Z => compile_reified_expr_Z locals v
+      | ?t => fail "Unrecognized type" t
+      end
+    end.
+
+  Ltac compile_reified_expr :=
+    compile_apply_expr_reification_lemma;
+    [ compile_prove_expr_reification_premise | .. ].
+End ExprReflection.
+
+Section with_parameters.
+  Context {semantics : Semantics.parameters}
+          {semantics_ok : Semantics.parameters_ok _}.
 
   Section NoSkips.
     Definition is_skip cmd :=
@@ -613,6 +998,11 @@ Section with_parameters.
 
     Definition compile_setup_remove_skips := noskips_correct.
   End NoSkips.
+End with_parameters.
+
+Section with_parameters.
+  Context {semantics : Semantics.parameters}
+          {semantics_ok : Semantics.parameters_ok _}.
 
   Section Setup.
     Definition wp_bind_retvars retvars (P: list word -> predicate) :=
@@ -779,17 +1169,6 @@ Ltac lookup_variable m val :=
   | map.put ?m' _ _ => lookup_variable m' val
   end.
 
-Ltac map_to_list m :=
-  let rec loop m acc :=
-      match m with
-      | map.put ?m ?k ?v =>
-        loop m uconstr:((k, v) :: acc)
-      | map.empty =>
-        (* Reverse for compatibility with map.of_list *)
-        uconstr:(List.rev acc)
-      end in
-  loop m uconstr:([]).
-
 Ltac solve_map_get_goal_refl m :=
   let b := map_to_list m in
   change m with (map.of_list b);
@@ -871,36 +1250,37 @@ Ltac compile_unfold_head_binder :=
   compile_unfold_head_binder' p.
 
 Create HintDb compiler.
-Hint Extern 1 => simple eapply compile_word_constant; shelve : compiler.
-Hint Extern 1 => simple eapply compile_word_of_Z_constant; shelve : compiler.
-Hint Extern 1 => simple eapply compile_Z_constant; shelve : compiler.
-Hint Extern 1 => simple eapply compile_nat_constant; shelve : compiler.
-Hint Extern 1 => simple eapply compile_bool_constant; shelve : compiler.
-Hint Extern 1 => simple eapply compile_word_add; shelve : compiler.
-Hint Extern 1 => simple eapply compile_word_sub; shelve : compiler.
-Hint Extern 1 => simple eapply compile_word_mul; shelve : compiler.
-Hint Extern 1 => simple eapply compile_word_mulhuu; shelve : compiler.
-Hint Extern 1 => simple eapply compile_word_divu; shelve : compiler.
-Hint Extern 1 => simple eapply compile_word_remu; shelve : compiler.
-Hint Extern 1 => simple eapply compile_word_and; shelve : compiler.
-Hint Extern 1 => simple eapply compile_word_or; shelve : compiler.
-Hint Extern 1 => simple eapply compile_word_xor; shelve : compiler.
-Hint Extern 1 => simple eapply compile_word_sru; shelve : compiler.
-Hint Extern 1 => simple eapply compile_word_slu; shelve : compiler.
-Hint Extern 1 => simple eapply compile_word_srs; shelve : compiler.
-Hint Extern 1 => simple eapply compile_Z_add; shelve : compiler.
-Hint Extern 1 => simple eapply compile_Z_sub; shelve : compiler.
-Hint Extern 1 => simple eapply compile_Z_mul; shelve : compiler.
-Hint Extern 1 => simple eapply compile_Z_and; shelve : compiler.
-Hint Extern 1 => simple eapply compile_Z_or; shelve : compiler.
-Hint Extern 1 => simple eapply compile_Z_xor; shelve : compiler.
-Hint Extern 1 => simple eapply compile_word_lts; shelve : compiler.
-Hint Extern 1 => simple eapply compile_word_ltu; shelve : compiler.
-Hint Extern 1 => simple eapply compile_word_eqb; shelve : compiler.
-Hint Extern 1 => simple eapply compile_bool_eqb; shelve : compiler.
-Hint Extern 1 => simple eapply compile_bool_andb; shelve : compiler.
-Hint Extern 1 => simple eapply compile_bool_orb; shelve : compiler.
-Hint Extern 1 => simple eapply compile_bool_xorb; shelve : compiler.
+Hint Extern 10 => simple eapply compile_word_constant; shelve : compiler.
+Hint Extern 10 => simple eapply compile_word_of_Z_constant; shelve : compiler.
+Hint Extern 10 => simple eapply compile_Z_constant; shelve : compiler.
+Hint Extern 10 => simple eapply compile_nat_constant; shelve : compiler.
+Hint Extern 10 => simple eapply compile_bool_constant; shelve : compiler.
+Hint Extern 10 => simple eapply compile_word_add; shelve : compiler.
+Hint Extern 10 => simple eapply compile_word_sub; shelve : compiler.
+Hint Extern 10 => simple eapply compile_word_mul; shelve : compiler.
+Hint Extern 10 => simple eapply compile_word_mulhuu; shelve : compiler.
+Hint Extern 10 => simple eapply compile_word_divu; shelve : compiler.
+Hint Extern 10 => simple eapply compile_word_remu; shelve : compiler.
+Hint Extern 10 => simple eapply compile_word_and; shelve : compiler.
+Hint Extern 10 => simple eapply compile_word_or; shelve : compiler.
+Hint Extern 10 => simple eapply compile_word_xor; shelve : compiler.
+Hint Extern 10 => simple eapply compile_word_sru; shelve : compiler.
+Hint Extern 10 => simple eapply compile_word_slu; shelve : compiler.
+Hint Extern 10 => simple eapply compile_word_srs; shelve : compiler.
+Hint Extern 10 => simple eapply compile_Z_add; shelve : compiler.
+Hint Extern 10 => simple eapply compile_Z_sub; shelve : compiler.
+Hint Extern 10 => simple eapply compile_Z_mul; shelve : compiler.
+Hint Extern 10 => simple eapply compile_Z_and; shelve : compiler.
+Hint Extern 10 => simple eapply compile_Z_or; shelve : compiler.
+Hint Extern 10 => simple eapply compile_Z_xor; shelve : compiler.
+Hint Extern 10 => simple eapply compile_word_lts; shelve : compiler.
+Hint Extern 10 => simple eapply compile_word_ltu; shelve : compiler.
+Hint Extern 10 => simple eapply compile_word_eqb; shelve : compiler.
+Hint Extern 10 => simple eapply compile_bool_eqb; shelve : compiler.
+Hint Extern 10 => simple eapply compile_bool_andb; shelve : compiler.
+Hint Extern 10 => simple eapply compile_bool_orb; shelve : compiler.
+Hint Extern 10 => simple eapply compile_bool_xorb; shelve : compiler.
+Hint Extern 8 => ExprReflection.compile_reified_expr; shelve : compiler. (* Higher priority than individual ops *)
 
 Ltac compile_binding :=
   (* We want to flip nlets before introducing nlet_eq. *)
@@ -908,7 +1288,7 @@ Ltac compile_binding :=
   (* We don't want to show users goals with nlet_eq, so compile_nlet_as_nlet_eq
      isn't in the ‘compiler’ hint db. *)
   try simple apply compile_nlet_as_nlet_eq;
-  progress unshelve (typeclasses eauto 3 with compiler); shelve_unifiable.
+  progress unshelve (typeclasses eauto with compiler); shelve_unifiable.
 
 (* Use [simple eapply] (not eapply) if you add anything here, to ensure that Coq
    doesn't peek past the first [nlet]. *)
